cleaner proofs

Lambda_Abstraction_in_VA_Calculus.v
@@ -31,18 +31,6 @@ Require Import Reflective.Rewriting_partI.
 Set Default Proof Using "Type".
 
 
-Ltac auto_t := eauto with TreeHintDb.
-Ltac eapply2 H := eapply H; auto_t.
-
-Ltac split_all := simpl; intros; 
-match goal with 
-| H : _ /\ _ |- _ => inversion_clear H; split_all
-| H : exists _, _ |- _ => inversion H; clear H; split_all 
-| _ =>  try (split; split_all); try contradiction
-end; try congruence; auto_t.
-
-Ltac exist x := exists x; split_all.
-
 (* Section 9.2: VA-Calculus *) 
 
 Inductive VA:  Set :=
@@ -342,10 +330,7 @@ Proof.  intros M N R; induction R; split_all. Qed.
 
 
 Lemma va_red_to_s_red: implies_red va_red s_red. 
-Proof. 
-eapply2 implies_red_multi_step. 
-red; split_all; one_step; eapply2 va_red1_to_s_red1. 
-Qed. 
+Proof. eapply2 implies_red_multi_step; red; split_all; one_step; eapply2 va_red1_to_s_red1. Qed. 
 
 Lemma to_va_red_multi_step: forall red, implies_red red va_red -> implies_red (multi_step red) va_red. 
 Proof. 
@@ -392,16 +377,58 @@ Proof. red; split_all; eapply2 diamond_va_red. Qed.
 
 
 Ltac zerotac := try eapply2 zero_red.
-Ltac succtac :=
-  repeat (eapply transitive_red;
-  [ eapply2 succ_red ;
-    match goal with
-    | |- multi_step va_red1 _ _ => idtac
-    | _ => fail (*gone too far ! *)
-    end
-  | ]); zerotac
-.
+Ltac succ1tac := repeat (eapply transitive_red; [ eapply2 succ_red ; fail (*gone too far ! *) | ]). 
+Ltac succtac := succ1tac; zerotac.
 Ltac aptac := eapply transitive_red; [ eapply preserves_app_va_red |].
+
+Ltac ap2tac:=
+  unfold va_red; 
+  eassumption || eapply2 Y2_red || 
+              match goal with
+              | |- multi_step _ (_ @ _) _ => try aptac; [ap2tac | ap2tac | ]
+              | _ => idtac
+              end. 
+Ltac vatac :=
+  unfold va_red; succ1tac; 
+  match goal with
+  | |- multi_step va_red1 Vop _ => zerotac
+  | |- multi_step va_red1 Lam _ => zerotac
+  | |- multi_step va_red1 (Vop @ _ @ _ @ _) _ => succtac
+  | |- multi_step va_red1 (Lam @ _ @ _ @ _) _ =>
+    eapply transitive_red;
+    [ eapply preserves_app_va_red ;
+      [ eapply preserves_app_va_red ;
+        [ eapply preserves_app_va_red ; [| vatac ] (* reduce the argument of △ *) 
+        | ]
+      | ]
+     |] ;
+    zerotac; (* put the "redex" back together *) 
+    match goal with
+   | |- multi_step va_red1 (Lam @ ?arg @ _ @ _) _ =>
+      match arg with
+      | Lam  => vatac (* made progress so recurse *) 
+      | Lam @ _  => vatac (* made progress so recurse *) 
+      | Lam @ _ @ _ => vatac (* made progress so recurse *) 
+      | _ => idtac (* no progress so stop *)
+      end
+    | _ => vatac (* for safety ? *) 
+    end 
+  | |- multi_step va_red1 (_ @ _) _ => (* not a ternary tree *) 
+    eapply transitive_red; [ eapply preserves_app_va_red ; vatac |] ; (* so reduce the function *)
+    match goal with
+    | |- multi_step va_red1 (Lam @ ?arg @ _ @ _) _ =>
+      match arg with
+      | Lam  => vatac (* made progress so recurse *) 
+      | Lam @ _  => vatac (* made progress so recurse *) 
+      | Lam @ _ @ _ => vatac (* made progress so recurse *) 
+      | _ => idtac (* no progress so stop *)
+      end
+    | _ => idtac
+    end
+  | _ => idtac (* the head is not △ *) 
+  end;
+  zerotac; succtac; zerotac. 
+      
 
 
 
@@ -653,34 +680,8 @@ Proof. intros; cbv; succtac. Qed.
 Lemma k_red : forall M N, va_red (Kop @ M @ N) M. 
 Proof.  intros; cbv; succtac. Qed. 
 
-
 Lemma sop_red: forall M N P, va_red (Sop @ M @ N @ P) (M@P@(N@P)). 
-Proof.
-  intros; cbv; succtac.
-  aptac;
-    [ aptac;
-      [ aptac;
-        [ aptac;
-          [ aptac; [ succtac | succtac | succtac]
-          | succtac
-          | zerotac]
-        | zerotac
-        | succtac]
-      | zerotac
-      | succtac]
-    | zerotac
-    | zerotac];
-    succtac; succtac; eapply2 preserves_app_va_red; aptac;
-      [ aptac;
-        [ aptac;
-          [ aptac;
-            [ zerotac | succtac | succtac]
-          | zerotac
-          | succtac]
-        | zerotac
-        | succtac] | |];
-      zerotac. 
-Qed.
+Proof.  intros; cbv; vatac. Qed.
 
 
   
@@ -688,7 +689,8 @@ Definition meaningful_translation_SK_to_VA f :=
   (forall M N, sk_red1 M N -> va_red (f M) (f N)) /\ (* strong version *) 
   (forall M N, f (Incompleteness_of_Combinatory_Logic.App M N) = App (f M) (f N)) /\  (* applications *) 
   (forall M, Incompleteness_of_Combinatory_Logic.program M -> valuable (f M)) /\ (* programs *) 
-  (forall i, f (Incompleteness_of_Combinatory_Logic.Ref i) = Ref i) .              (* variables *) 
+  (forall i, f (Incompleteness_of_Combinatory_Logic.Ref i) = Ref i)               (* variables *) 
+.
 
 Fixpoint sk_to_va M :=
   match M with
@@ -726,24 +728,19 @@ Proof.
     | intros M prM; induction prM].   
   { exists Sop;   split; [ apply zero_red | cbv; auto; program_tac]. }
   {
-  elim IHprM; intro x; split_all. repeat eexists. 
-  unfold Sop, v, env_comb. aptac. 2: eassumption. zerotac.
-  aptac. succtac.   zerotac. aptac.  aptac. aptac. zerotac. succtac. succtac. succtac. succtac.
-  succtac. eapply transitive_red.  succtac.
-  aptac. zerotac. succtac. succtac. program_tac.
+  elim IHprM; split_all; repeat eexists;  
+    [ eapply transitive_red; [ap2tac; zerotac | unfold Sop, v, env_comb; vatac ]
+    | program_tac].
   }{
-  elim IHprM1; intro x; split_all; elim IHprM2; intro x0; split_all. 
-   red. repeat eexists.  aptac. aptac. zerotac. eassumption. zerotac. eassumption. 
-  unfold Sop, v, env_comb. aptac. aptac. aptac. aptac. zerotac. succtac. succtac. zerotac.
-  succtac.   zerotac. succtac. zerotac.
-  aptac. aptac. zerotac. aptac. aptac. zerotac. succtac. succtac. succtac. succtac. succtac. zerotac.
-  eapply transitive_red. succtac.  aptac. zerotac. aptac. aptac. zerotac. aptac. zerotac. aptac. succtac.
-  succtac. succtac. succtac. succtac. succtac. succtac. succtac. program_tac. 
+  elim IHprM1;split_all;  elim IHprM2; split_all;  repeat eexists; 
+    [ eapply transitive_red; [ap2tac; zerotac | unfold Sop, v, env_comb; vatac ]
+    | program_tac].
   }
   {exist Kop; unfold Kop, v; cbv; program_tac. }
   {
-    elim IHprM; intro x; split_all; repeat eexists;
-      [ aptac; [ zerotac | eassumption | unfold Kop, v; succtac] |  program_tac].
+    elim IHprM; split_all; repeat eexists;
+    [ eapply transitive_red; [ap2tac; zerotac | unfold Kop; vatac ]
+    | program_tac].
   }
 Qed.
 
@@ -928,8 +925,7 @@ Lemma pentagon_id_red_s_ranked:
                                               s_ranked n N Q2 .
 Proof.
   induction m; intros M P r N ir; inversion r; clear r; subst; eauto.
-  (* 2 *)
-  exists 0; exists P; exist N; exist 0; repeat split; auto. 
+  { exists 0, P, N; exist 0. } 
   (* 1 *)
   assert(pent: exists Q1 Q2,  s_red N0 Q1 /\ id_red Q1 Q2 /\  s_red N Q2) by 
   eapply2 pentagon_id_red_s_red1.
@@ -952,14 +948,13 @@ Lemma pentagon_id_red_s_red:
                          exists Q1 Q2,  s_red P Q1 /\ id_red Q1 Q2 /\
                                         s_red N Q2 .
 Proof.
-  intros M P r N idr. 
-  elim(s_red_implies_s_ranked _ _ r); intros.   
+  intros M P r N idr; 
+  elim(s_red_implies_s_ranked _ _ r); intros;    
   assert(pent: exists p Q1 Q2 n,  s_ranked p P Q1 /\ id_red Q1 Q2 /\ s_ranked n N Q2)
-    by eapply2 pentagon_id_red_s_ranked.
-  elim pent. intros p; clear pent. intro pent2; elim pent2; intros Q1 pent3; clear pent2.
-  elim pent3; intros Q2 n; clear pent3;  split_all. 
-  exists Q1; exist Q2.
-  all: eapply2 s_ranked_implies_s_red. 
+    by eapply2 pentagon_id_red_s_ranked; 
+  elim pent;  intros p; clear pent;  intro pent2; elim pent2; intros Q1 pent3; clear pent2; 
+  elim pent3; intros Q2 n; clear pent3;  split_all;  
+  exists Q1; exist Q2; eapply2 s_ranked_implies_s_red. 
 Qed.
 
   (* 
@@ -974,32 +969,32 @@ Lemma triangle_id_red_s_red_ref:
             forall N, id_red M N ->
                       s_red N (Ref x) .
 Proof.
-  intros M x r N ir.
+  intros M x r N ir;
   assert(pent: exists Q1 Q2,  s_red (Ref x) Q1 /\ id_red Q1 Q2 /\
-                              s_red N Q2) by  eapply2 pentagon_id_red_s_red.
-  elim pent. intros Q1 pent2; clear pent.
-  elim pent2; intro Q2; clear pent2; split_all.
-  assert(Q1 = Ref x) by eapply2 refs_are_stable; subst.
+                              s_red N Q2) by  eapply2 pentagon_id_red_s_red;
+  elim pent; intros Q1 pent2; clear pent;
+  elim pent2; intro Q2; clear pent2; split_all;
+  assert(Q1 = Ref x) by eapply2 refs_are_stable; subst;
   inv id_red.   
 Qed.
 
 
 Theorem equality_of_programs_is_not_definable_in_va:  forall eq,  not (is_equal eq). 
 Proof.
-  intros; intro premise; inversion premise as (eq0 & eq1). 
-  assert(r: s_red (eq @ Iop @ (Lam @ Vop @ Iop) @ (Ref "x") @ (Ref "y")) (Ref "y")).
-  eapply va_red_to_s_red. eapply2 premise. cbv; program_tac. cbv; program_tac. discriminate. 
+  intros; intro premise; inversion premise as (eq0 & eq1); 
+  assert(r: s_red (eq @ Iop @ (Lam @ Vop @ Iop) @ (Ref "x") @ (Ref "y")) (Ref "y")) by  
+  (eapply va_red_to_s_red; eapply2 premise; [cbv; program_tac | cbv; program_tac | discriminate]);  
   elim(pentagon_id_red_s_red (eq @ Iop @ (Lam @ Vop @ Iop) @ (Ref "x") @ (Ref "y")) (Ref "y")
-                                  r (eq @ Iop @ Iop @ (Ref "x") @ (Ref "y"))); split_all. 
-  2: repeat eapply2 id_app; eapply2 id_red_refl. 
-  assert(x = Ref "y") by eapply2 refs_are_stable. subst. 
-  inv id_red.   
-  assert (r2: s_red (eq @ Iop @ Iop @ (Ref "x") @ (Ref "y")) (Ref "x")).
-  eapply2 va_red_to_s_red.
-  eapply2 eq0. cbv; program_tac. 
-  elim(diamond_s_red _ _ r2 (Ref "y")); auto.  intros x (s1&s2).
-  assert(x = Ref "x") by eapply2 refs_are_stable. 
-  assert(x = Ref "y") by eapply2 refs_are_stable. subst; discriminate. 
+                                  r (eq @ Iop @ Iop @ (Ref "x") @ (Ref "y"))); split_all;
+    [
+      assert(x = Ref "y") by eapply2 refs_are_stable;  subst;  inv id_red;   
+      assert (r2: s_red (eq @ Iop @ Iop @ (Ref "x") @ (Ref "y")) (Ref "x")) by
+          (eapply2 va_red_to_s_red;  eapply2 eq0; cbv; program_tac); 
+      elim(diamond_s_red _ _ r2 (Ref "y")); auto;  intros x (?&?); 
+      assert(x = Ref "x") by eapply2 refs_are_stable; 
+      assert(x = Ref "y") by eapply2 refs_are_stable; subst; discriminate
+    | repeat eapply2 id_app; eapply2 id_red_refl
+    ]. 
 Qed.
 
 
@@ -1024,18 +1019,11 @@ Definition getTag := (* \"" (Lam @ (Ref "") @ Iop @ KI @ Lam). *)
 
 
 Lemma tag_apply : forall t f x, va_red (tag t f @ x) (f @ x).
-Proof.
-  intros.  unfold tag, ndx. succtac. aptac. aptac. aptac.  eapply2 env_zero_red.
-  zerotac. eapply2 env_zero_red. aptac. eapply2 env_succ_red. zerotac.
-  aptac. eapply2 env_nil_red. all: zerotac. unfold Kop;  succtac. 
-Qed.
+Proof.  intros; cbv; vatac. Qed.
 
 
 Lemma getTag_tag : forall t f, va_red (getTag @ (tag t f)) t.
-Proof.
-  intros. cbv; succtac. aptac. aptac. aptac. aptac. aptac. succtac.  succtac. succtac.
-  succtac. succtac.  succtac. succtac.  succtac. succtac. succtac. succtac.
-Qed.
+Proof.  intros;  cbv; vatac. Qed.
 
 Lemma tag_preserves_substitute:
   forall t f x N, substitute (tag t f) x N = tag (substitute t x N) (substitute f x N). 
@@ -1057,36 +1045,17 @@ Definition stem x :=
 
    
 Lemma stem_red : forall x y z,  va_red (App (App (stem x) y) z) (App (App y z) (App x z)).
-Proof.
-  intros; cbv; succtac. aptac. aptac. aptac. aptac. aptac. succtac. succtac. succtac.
-  zerotac.  succtac. zerotac. succtac. zerotac. zerotac. succtac.
-  eapply2 preserves_app_va_red.
-  aptac. aptac. aptac. aptac. zerotac. succtac. succtac. zerotac. succtac. zerotac. succtac.
-  all: zerotac.
-Qed. 
+Proof.  intros; cbv; vatac. Qed. 
 
 Lemma valuable_stem: forall x, valuable x -> valuable (stem x).
 Proof.
-  unfold valuable; split_all. exist (stem x0).
-  cbv; repeat eapply2 preserves_app_va_red. cbv; program_tac. 
+  unfold valuable; split_all; exist (stem x0); cbv; [repeat eapply2 preserves_app_va_red | program_tac]. 
 Qed.
 
-Definition fork x y :=
-  Lam
-    @  (Lam
-          @ (v (v (ndx 0) @ (v x)) @ (v y))
-          @ Iop
-       )
-    @ Iop
-    . 
+Definition fork x y := Lam @  (Lam @ (v (v (ndx 0) @ (v x)) @ (v y)) @ Iop) @ Iop. 
 
-
-  
 Lemma fork_red: forall w x y z, va_red (App (App (fork w x) y) z) (App (App z w) x).
-Proof.
-  intros; unfold fork, ndx, env_comb; succtac.
-  eapply2 preserves_app_va_red. eapply2 preserves_app_va_red. all: cbv; succtac.
-Qed.  
+Proof.  intros; cbv; vatac. Qed.  
 
 Lemma substitution_stem :
   forall f x N, (substitute (stem f) x N) = stem (substitute f x N).
@@ -1100,8 +1069,7 @@ Proof. intros; cbv; auto. Qed.
 
 Lemma valuable_fork: forall x y, valuable x -> valuable y -> valuable (fork x y).
 Proof.
-  unfold valuable; split_all. exist (fork x1 x0).
-  cbv; repeat eapply2 preserves_app_va_red. cbv; program_tac. 
+  unfold valuable; split_all; exist (fork x1 x0); cbv; [repeat eapply2 preserves_app_va_red | program_tac]. 
 Qed.
 
 
@@ -1113,10 +1081,10 @@ Lemma substitute_preserves_va_red:
   forall M M', va_red M M' -> forall x N, va_red (substitute M x N) (substitute M' x N).
 Proof.
   cut(forall red M M', multi_step red M M' -> red = va_red1 ->
-                       forall x N, va_red  (substitute M x N) (substitute M' x N)).
-  intro aux;  intros.  eapply2 aux.
-  intros red M M' r; induction r; split_all; subst.
-  eapply succ_red. eapply2 substitute_preserves_va_red1. eapply2 IHr.
+                       forall x N, va_red  (substitute M x N) (substitute M' x N)); 
+  [ intro aux;  intros;  eapply2 aux
+  | intros red M M' r; induction r; split_all; subst; 
+    eapply succ_red; [ eapply2 substitute_preserves_va_red1 | eapply2 IHr]].
 Qed.
 
 (* 
@@ -1157,12 +1125,7 @@ Lemma kernel1_red :
                    "x" x))
  
 .
-Proof.
-  intros x; unfold kernel; succtac. eapply transitive_red. eapply2 tag_apply.
-  eapply transitive_red.  eapply2 star_beta. 
-  rewrite ! tag_preserves_substitute.    rewrite substitution_stem. unfold substitute; fold substitute.
-  rewrite eqb_refl.  zerotac. 
-Qed.
+Proof.  intros; cbv; vatac.  Qed.
 
 
 Lemma kernel2_red :
@@ -1176,45 +1139,45 @@ Lemma kernel2_red :
      (Lam @ Vop @ Lam))
           ).
 Proof.
-  intros x y.   aptac. eapply2 kernel1_red.   zerotac.
-  eapply transitive_red. eapply2 tag_apply.
-  unfold tag, fork, star, star_body; fold star_body. simpl.  
-  succtac. eapply2 preserves_app_va_red.   succtac. eapply2 preserves_app_va_red.
-  eapply2 preserves_app_va_red.   eapply2 preserves_app_va_red. succtac. 
-  eapply2 preserves_app_va_red.   eapply2 preserves_app_va_red. succtac. 
-  eapply2 preserves_app_va_red.   eapply2 preserves_app_va_red. succtac. 
-  eapply2 preserves_app_va_red.   succtac. eapply2 preserves_app_va_red. succtac.
-  eapply2 preserves_app_va_red.   succtac.
-  eapply2 preserves_app_va_red.   eapply2 preserves_app_va_red.   succtac. eapply2 preserves_app_va_red.
-  succtac.   eapply2 preserves_app_va_red.   succtac. eapply2 preserves_app_va_red. succtac. 
+  intros x y;   aptac;
+    [ eapply2 kernel1_red
+    | zerotac
+    | eapply transitive_red;
+      [ eapply2 tag_apply
+      | unfold tag, fork, star, star_body; fold star_body;  simpl; succtac; 
+        repeat ( eapply2 preserves_app_va_red; succtac)]].
 Qed.
 
 
 Lemma kernel3_red:  forall x y z, va_red (kernel @ x @ y @ z) (getTag @ x @ y @ z).
 Proof.
-  intros x y z.  aptac. eapply2 kernel2_red. zerotac.
-  eapply transitive_red. eapply2 tag_apply. succtac. eapply2 preserves_app_va_red.
-  eapply2 preserves_app_va_red. succtac. 
+  intros x y z;  aptac;
+    [eapply2 kernel2_red
+    | zerotac
+    | eapply transitive_red;
+      [ eapply2 tag_apply
+      | succtac;  eapply2 preserves_app_va_red; eapply2 preserves_app_va_red;  succtac]]. 
 Qed.
 
 
 Lemma get_tag_kernel_red:
   forall y z, va_red (App (App (App getTag kernel) y) z) y.
-Proof. intros x y; unfold kernel.  aptac. aptac.  eapply2 getTag_tag. all: zerotac. cbv; succtac. Qed. 
+Proof. intros x y; unfold kernel;  aptac; [ aptac; [eapply2 getTag_tag | |] | |]; zerotac; cbv; succtac. Qed. 
 
 Lemma get_tag_stem_red:
   forall x y z, va_red (getTag @ (kernel @ x) @ y @ z) (y @ z @ (x @ z)). 
 Proof.
-  intros x y z; intros; aptac. aptac. aptac. zerotac. eapply2 kernel1_red.
-  eapply2 getTag_tag. all: zerotac. eapply2 stem_red.   
+  intros x y z; intros; aptac;
+    [aptac; [aptac; [zerotac | eapply2 kernel1_red | eapply2 getTag_tag] | |] | |];
+    zerotac; eapply2 stem_red.   
 Qed.
 
 
 Lemma get_tag_fork_red:
   forall w x y z, va_red (getTag @ (kernel @ w @ x) @ y @ z) (z @ w @ x). 
 Proof.
-  intros w x y z. intros. aptac. aptac. aptac.  zerotac. eapply2 kernel2_red. all: zerotac.
-  cbv; repeat eapply2 is_App.   aptac. aptac.   eapply2 getTag_tag. all: zerotac.   cbv; succtac.   
+  intros w x y z; intros; aptac; [ aptac; [ aptac; [zerotac | eapply2 kernel2_red | ] | |] | |]; zerotac; 
+  cbv; repeat eapply2 is_App;   aptac; [ aptac; [ eapply2 getTag_tag | |] | |]; zerotac; cbv; succtac.   
 Qed.
 
 
@@ -1237,23 +1200,25 @@ Fixpoint tree_to_va M :=
 Lemma preserves_reduction1_tree_to_va:
   forall M N, t_red1 M N -> va_red (tree_to_va M) (tree_to_va N).
 Proof.
-  assert(combination getTag) by repeat eapply2 is_App. 
+  assert(combination getTag) by repeat eapply2 is_App;  
   intros M N r; induction r; subst; split_all.
-  (* 5 *) 
-  4,5: eapply2 preserves_app_va_red.
-  (* 3 *)
-  eapply transitive_red. eapply2 kernel3_red.  eapply2 get_tag_kernel_red. 
-  (* 2 *) 
-  eapply transitive_red. eapply2 kernel3_red.
-  aptac. aptac. aptac.    zerotac. eapply2 kernel1_red. 
-  eapply2 getTag_tag.   all: zerotac. eapply2 stem_red.   
-  (* 1 *)
-  eapply transitive_red. eapply2 kernel3_red.
-  aptac. aptac. aptac.    zerotac. eapply2 kernel2_red. 
-  eapply2 getTag_tag.   all: zerotac.  cbv; succtac. 
+  { eapply transitive_red; [ eapply2 kernel3_red |  eapply2 get_tag_kernel_red]. } 
+  {
+    eapply transitive_red;
+      [ eapply2 kernel3_red
+      | aptac; [ aptac; [ aptac; [ zerotac | eapply2 kernel1_red | eapply2 getTag_tag] | |] | |];
+        zerotac;  eapply2 stem_red].
+    }
+  {
+    eapply transitive_red;
+      [ eapply2 kernel3_red
+      | aptac; [ aptac; [ aptac; [ zerotac | eapply2 kernel2_red | eapply2 getTag_tag] | |] | |]; zerotac];
+      cbv; succtac.
+  }
+ all: eapply2 preserves_app_va_red. 
 Qed.
 
-
+(* clean proofs to here *) 
 
 Lemma preserves_reduction_tree_to_va:
   forall M N, t_red M N -> va_red (tree_to_va M) (tree_to_va N).
@@ -1289,11 +1254,13 @@ Proof.
   cbv; program_tac.
   eauto.
   (* 1 *)
-  subst. repeat eexists. 
-  aptac. aptac. zerotac. eassumption.  zerotac. eassumption.
-  eapply transitive_red. eapply2 kernel2_red.  eapply va_red_preserves_tags. zerotac.
-  aptac. aptac. zerotac. aptac. aptac. zerotac. aptac. zerotac. succtac. all: zerotac.
-  cbv; program_tac.
+  subst; repeat eexists;
+    [eapply transitive_red;
+     [ap2tac; zerotac
+     | eapply transitive_red;
+       [eapply2 kernel2_red
+       | eapply va_red_preserves_tags; [ zerotac | vatac]]]
+    | cbv; program_tac].
 Qed.
 
 
@@ -1301,11 +1268,7 @@ Qed.
   
 Theorem meaningful_translation_from_tree_to_va:
   meaningful_translation_tree_to_va tree_to_va. 
-Proof.
-  split_all. 
-  eapply2 preserves_reduction1_tree_to_va.
-  elim(valuable_trees M); split_all.   exist x. 
-Qed.
+Proof. split_all; [eapply2 preserves_reduction1_tree_to_va |elim(valuable_trees M); split_all; exist x]. Qed.
 
 (* 
 Compute (term_size kernel). = 200 
@@ -1474,32 +1437,13 @@ Lemma programmable_getTag1_Lamt2:
               programmable (getTag1 (Lam_t @ M@N) @ (K @ (K @ Lam_t))).
 Proof.
   unfold programmable; split_all; repeat eexists;
-      [ eapply transitive_red;
-        [unfold getTag1; eapply transitive_red;
-           [aptac;
-            [aptac;
-             [ aptac;
-               [ aptac;
-                 [ zerotac
-                 | aptac;
-                   [ aptac;
-                     [ aptac;
-                       [ aptac;
-                         [ zerotac
-                         | aptac; [ eapply2 Y2_red | zerotac | zerotac]; trtac
-                         | fold Lam_t;  unfold Lam_0; trtac]                 
-                       | | ]
-                     | |]
-                   | |]
-                 | ]
-               | |]
-             | |]
-            | |]; 
-            zerotac; trtac
-           | aptac; [ trtac | zerotac | zerotac]]  
-        | aptac;  [ trtac | zerotac | eapply transitive_red; [ trtac | ap2tac; zerotac]]
-        ]
-      | program_tac].
+    [ eapply transitive_red;
+      [ ap2tac; zerotac
+      | assert(t_red (Lam_t @ M) (Lam_0 @ Lam_t @ x2)) by
+          (eapply transitive_red; [eapply2 Y2_red | ap2tac; zerotac]); 
+        unfold getTag1; eapply transitive_red; [ ap2tac; zerotac |]];
+      eapply transitive_red; [ unfold Lam_0; trtac | aptac; [ trtac | trtac | trtac]]
+    | program_tac].
 Qed.
 
 Lemma programmable_getTag1_Lamt2_app:
@@ -1520,6 +1464,9 @@ Qed.
 
 
 
+Ltac Vt_tac x :=
+  assert(t_red (V_t @ x) (V_0 @ V_t @ x)) by eapply2 Y2_t_red;
+  unfold getTag1; eapply transitive_red; [ ap2tac; zerotac | unfold V_0; trtac];  trtac. 
 
 
 
@@ -1531,95 +1478,40 @@ Proof. intros; cbv; trtac. Qed.
 Lemma V_t1_red :
   forall x f sigma,
     t_red (getTag1 (V_t @ x) @ f @ sigma) (d (K@ x) @ (K@sigma)). 
-Proof.
-  intros; unfold getTag1; trtac;
-    aptac;
-    [aptac;
-     [aptac;
-      [ aptac;
-        [ aptac;
-          [ zerotac
-          | aptac;
-            [ aptac;
-              [ aptac;
-                [ aptac;
-                  [ zerotac
-                  | eapply2 Y2_t_red
-                  | fold V_t;  unfold V_0; trtac]                 
-                | | ]
-              | |]
-            | |]
-          | ]
-        | |]
-      | |]
-     | |]
-    | |]; 
-    zerotac; trtac. 
-Qed.
+Proof.  intro x; intros; Vt_tac x. Qed.
 
 Lemma V_t2_red :
   forall x y sigma,
     t_red (getTag1 (V_t @ x @ y) @ (K@(K@ Lam_t)) @ sigma)
           (d (Lam_t @ y @ sigma) @ (Lam_t @ x @ sigma)). 
-Proof.
-  intros; unfold getTag1; trtac;
-    aptac;
-    [aptac;
-     [aptac;
-      [ aptac;
-        [ aptac;
-          [ zerotac
-          | aptac;
-            [ aptac;
-              [ aptac;
-                [ aptac;
-                  [ zerotac
-                  | aptac;
-                    [ eapply2 Y2_t_red
-                    | zerotac
-                    | fold V_t;  unfold V_0; trtac]
-                  |]
-                | | ]
-              | |]
-            | |]
-          | ]
-        | |]
-      | |]
-     | |]
-    | |]; 
-    zerotac; trtac. 
-Qed.
+Proof.  intro x; intros; Vt_tac x. Qed.
+
 
 
 Lemma V_t3_red: forall x y z, t_red (V_t @ x @ y @ z) (V_t @ (V_t @ x @ y) @ z). 
-Proof.
-  intros. aptac. aptac. eapply2 Y2_t_red. zerotac.  fold V_t. unfold V_0. 
-  do 5 (eapply transitive_red; [eapply2 succ_red | ]).
-  aptac. aptac. aptac. aptac. zerotac. trtac. all: zerotac.  trtac.
-Qed.
+Proof.  intro x; intros; Vt_tac x. Qed.
 
 
 Lemma Lam_t_V_t0_red : forall y z, t_red (Lam_t @ V_t @ y @ z) z.
-Proof.  intros. eapply transitive_red. eapply2 Lam_t3_red. unfold V_t, Y2_t, tag, getTag1, d;  trtac. Qed.
+Proof.  intros; eapply transitive_red; [ eapply2 Lam_t3_red | unfold V_t, Y2_t, tag, getTag1, d; trtac]. Qed.
 
 Lemma Lam_t_V_t_red : forall x y z, t_red (Lam_t @ (V_t @ x) @ y @ z) (y@x).
 Proof.
-  intros. eapply transitive_red. eapply2 Lam_t3_red.  unfold V_t, Y2_t, getTag1, tag, d.  trtac.
-    aptac. aptac. aptac. aptac. aptac. aptac. zerotac. aptac. aptac. aptac. aptac. zerotac.
-    eapply2 wait_red. unfold self_apply. trtac. all: zerotac.
-    unfold V_0 at 1; unfold tag_wait; trtac.
-    aptac. aptac. aptac. aptac. aptac. aptac. zerotac. trtac. all: zerotac. trtac.
+  intros; eapply transitive_red;
+    [ eapply2 Lam_t3_red
+    | unfold V_t, Y2_t, tag, getTag1, d; trtac; unfold wait, self_apply, d, V_0; trtac; 
+      aptac; [ trtac | zerotac | trtac]].
 Qed.
 
 Lemma Lam_t_V_t2_red :
   forall x y z w, t_red (Lam_t @ (V_t @ w @ x) @ y @ z) (Lam_t @ w @ y @ z @ (Lam_t @ x @ y @ z)).
 Proof.
-  intros. eapply transitive_red. eapply2 Lam_t3_red.  unfold V_t, Y2_t, getTag1, tag, d.  trtac.
-    aptac. aptac. aptac. aptac. aptac. aptac. zerotac. aptac. aptac. aptac. aptac. zerotac.
-    aptac.  eapply2 wait_red. all: zerotac.  unfold self_apply.  starstac ("x" :: nil).
-     unfold V_0 at 1; unfold tag_wait; trtac.
-    aptac. aptac. aptac. aptac. aptac. aptac. zerotac. trtac. all: zerotac. trtac.
+  intros; eapply transitive_red;
+    [ eapply2 Lam_t3_red
+    | unfold V_t, Y2_t, tag, getTag1, d; trtac; unfold wait, self_apply, d, V_0; trtac; 
+      aptac; [ trtac | zerotac | trtac]].
 Qed.
+
 
 
 
@@ -1634,30 +1526,25 @@ Fixpoint va_to_tree M :=
     
 Lemma preserves_combination_ac_to_tree:
   forall M, Lambda_Abstraction_in_VA_Calculus.combination M -> combination (va_to_tree M).
-Proof.  intros M c; induction c; zerotac; cbv; auto 1000 with *. Qed.
+Proof.  intros M c; induction c; zerotac; cbv; auto 1000 with TreeHintDb. Qed.
 
 
 Lemma preserves_reduction1_va_to_tree:
   forall M N, va_red1 M N -> t_red (va_to_tree M) (va_to_tree N).
 Proof.
   intros M N r; induction r; subst; split_all;
-    try (eapply2 preserves_app_t_red; zerotac; fail).
-  (* 7 *)
-  eapply2 V_t3_red. 
-  eapply2 Lam_t_V_t0_red.
-  eapply2 Lam_t_V_t_red.
-  eapply2 Lam_t_V_t2_red.
-  (* 3 *) 
-  eapply transitive_red. eapply2 Lam_t3_red. aptac. aptac. aptac. instantiate(1:= Id). cbv; trtac.
-  zerotac. trtac.  trtac. trtac. trtac. trtac.
-  (* 2 *)
-  eapply transitive_red. eapply2 Lam_t3_red. aptac. aptac. aptac. aptac. aptac. aptac.
-  zerotac. aptac. aptac. aptac. aptac. zerotac. 
-  eapply2 Y2_red.   fold Lam_t. unfold Lam_0; trtac. all: zerotac. trtac.
-  (* 1 *)
-  eapply transitive_red. eapply2 Lam_t3_red. aptac. aptac. aptac. aptac. aptac. aptac.
-  zerotac. aptac. aptac. aptac. aptac. zerotac.  aptac. 
-  eapply2 Y2_red.   zerotac. fold Lam_t. unfold Lam_0; trtac. all: zerotac. trtac.
+    try (eapply2 preserves_app_t_red; zerotac; fail);
+  [
+    eapply2 V_t3_red 
+  | eapply2 Lam_t_V_t0_red
+  | eapply2 Lam_t_V_t_red
+  | eapply2 Lam_t_V_t2_red
+  | eapply transitive_red; [ eapply2 Lam_t3_red |  cbv; trtac] | |];
+  (eapply transitive_red;
+  [eapply2 Lam_t3_red
+  | unfold getTag1;  
+    assert(t_red (Lam_t @ (va_to_tree M)) (Lam_0 @ Lam_t@ va_to_tree M)) by eapply2  Y2_red; 
+    eapply transitive_red; [ ap2tac; zerotac |  unfold Lam_0; trtac; aptac; [ trtac | zerotac | trtac]]]).
 Qed.
 
 Ltac prog_aux_tac :=  repeat eexists;
@@ -1681,30 +1568,11 @@ Lemma programmable_getTag1_Vt1:
   forall M, programmable M -> programmable (getTag1 (V_t @ M) @ (K @ (K @ Lam_t))).
 Proof.
   intros M prM; inversion prM as [M1 (?&?)]; repeat eexists; 
-    [ unfold getTag1; eapply transitive_red;
-      [ap2tac; zerotac  
-      | eapply transitive_red;
-        [aptac;
-         [aptac;
-          [ aptac;
-            [ aptac;
-              [ zerotac
-              | aptac;
-                [ aptac;
-                  [ aptac;
-                    [ aptac;
-                      [ zerotac
-                      | eapply2 Y2_t_red
-                      | fold V_t;  unfold V_0; trtac]                 
-                    | | ]
-                  | |]
-                | |]
-              | ]
-            | |]
-          | |]
-         | |]; 
-         zerotac; trtac
-        | aptac; [ trtac | zerotac | trtac]]]
+    [ assert(t_red (V_t @ M) (V_0 @V_t@ M1)) by
+        (eapply transitive_red; [eapply2  Y2_t_red | ap2tac; zerotac]);   
+      unfold getTag1; eapply transitive_red;
+      [ap2tac; zerotac
+      | eapply transitive_red;  [ unfold V_0; trtac | aptac; [ trtac | zerotac | trtac]]]
     | program_tac]. 
 Qed. 
 
@@ -1719,15 +1587,12 @@ Qed.
 Lemma programmable_Vt2: forall M N, programmable M -> programmable N -> programmable (V_t @ M@ N).
 Proof.
   intros M N prM prN; inversion prM as [M1 (?&?)]; inversion prN as [N1 (?&?)]; repeat eexists;  
-    [ ap2tac;
-      [zerotac
-      |zerotac  
-      | eapply transitive_red;
-        [ aptac;
-          [ eapply2 Y2_t_red | zerotac | fold V_t; unfold V_0; trtac]
-        | aptac; [ trtac | zerotac | trtac]
-      ] ]
-    |  program_tac ]. 
+    [ assert(t_red (V_t @ M) (V_0 @V_t@ M1)) by
+        (eapply transitive_red; [eapply2  Y2_t_red | ap2tac; zerotac]);   
+      unfold getTag1; eapply transitive_red;
+      [ap2tac; zerotac
+      | eapply transitive_red;  [ unfold V_0; trtac | aptac; [ trtac | zerotac | trtac]]]
+    | program_tac]. 
 Qed. 
 
 
@@ -1736,34 +1601,15 @@ Lemma programmable_getTag1_Vt2:
               programmable (getTag1 (V_t @ M@N) @ (K @ (K @ Lam_t))).
 Proof.
   intros M N prM prN;
-    inversion prM as [M1 (?&?)]; inversion prN as [N1 (?&?)]; repeat eexists;
-      [ eapply transitive_red;
-        [unfold getTag1; eapply transitive_red;
-         [ap2tac; zerotac  
-         | eapply transitive_red;
-           [aptac;
-            [aptac;
-             [ aptac;
-               [ aptac;
-                 [ zerotac
-                 | aptac;
-                   [ aptac;
-                     [ aptac;
-                       [ aptac;
-                         [ zerotac
-                         | aptac; [ eapply2 Y2_t_red | zerotac | zerotac]; trtac
-                         | fold V_t;  unfold V_0; trtac]                 
-                       | | ]
-                     | |]
-                   | |]
-                 | ]
-               | |]
-             | |]
-            | |]; 
-            zerotac; trtac
-           | aptac; [ trtac | zerotac | zerotac]]]  
-        | aptac;  [ trtac | zerotac | eapply transitive_red; [ trtac | ap2tac; zerotac]]
-        ]
+    inversion prM as [M1 (?&?)]; inversion prN as [N1 (?&?)]; repeat eexists; 
+    [ assert(t_red (V_t @ M) (V_0 @V_t@ M)) by eapply2  Y2_t_red;   
+      unfold getTag1; eapply transitive_red;
+      [ap2tac; zerotac
+      | eapply transitive_red;
+        [ unfold V_0; trtac
+        | eapply transitive_red;
+          [aptac; [ trtac | zerotac | trtac]
+          | ap2tac; zerotac]]]
       | program_tac].
 Qed. 
 
@@ -1818,8 +1664,4 @@ Definition meaningful_translation_ac_to_tree (f: VA -> Tree) :=
   
 Theorem meaningful_translation_from_ac_to_tree:
   meaningful_translation_ac_to_tree va_to_tree. 
-Proof.
-  split_all. 
-  eapply2 preserves_reduction1_va_to_tree.
-  eapply2 preserves_programs_va_to_tree. 
-Qed.
+Proof. split_all; [eapply2 preserves_reduction1_va_to_tree | eapply2 preserves_programs_va_to_tree]. Qed.
